GraphQL/NormalForm/GroundTypeNormalization/FieldCollection.lean
@@ -14,6 +14,8 @@ namespace NormalForm
 
 namespace GroundTypeNormalization
 
+variable {ObjectIdentity : Type}
+
 theorem executableFieldScoped?_some
     {schema : Schema} {field : Execution.ExecutableField}
     {scopedField : FieldMerge.ScopedField} :
@@ -127,7 +129,7 @@ theorem typeIncludesObjectBool_eq_of_objectTypeNameBool_true_for_collection
 
 theorem doesFragmentTypeApplyBool_eq_typesOverlapBool_of_object_parent_source
     (schema : Schema) {parentType typeCondition : Name}
-    {source : Execution.Value} :
+    {source : Execution.Value ObjectIdentity} :
     objectTypeNameBool schema parentType = true ->
       (∃ runtimeType identity,
         source = .object runtimeType identity
@@ -1001,13 +1003,13 @@ theorem withoutExecutableGroupsWithResponseName_namesNodup
 
 theorem collectFields_nil
     (schema : Schema) (variableValues : Execution.VariableValues)
-    (parentType : Name) (source : Execution.Value) :
+    (parentType : Name) (source : Execution.Value ObjectIdentity) :
     Execution.collectFields schema variableValues parentType source [] = [] := by
   rfl
 
 theorem collectFields_cons
     (schema : Schema) (variableValues : Execution.VariableValues)
-    (parentType : Name) (source : Execution.Value)
+    (parentType : Name) (source : Execution.Value ObjectIdentity)
     (selection : Selection) (rest : List Selection) :
     Execution.collectFields schema variableValues parentType source
       (selection :: rest)
@@ -1019,7 +1021,7 @@ theorem collectFields_cons
 
 theorem collectFields_field_noDirectives
     (schema : Schema) (variableValues : Execution.VariableValues)
-    (parentType : Name) (source : Execution.Value)
+    (parentType : Name) (source : Execution.Value ObjectIdentity)
     (responseName fieldName : Name) (arguments : List Argument)
     (selectionSet rest : List Selection) :
     Execution.collectFields schema variableValues parentType source
@@ -1038,7 +1040,7 @@ theorem collectFields_field_noDirectives
 
 theorem collectFields_inlineFragment_none_directiveFree
     (schema : Schema) (variableValues : Execution.VariableValues)
-    (parentType : Name) (source : Execution.Value)
+    (parentType : Name) (source : Execution.Value ObjectIdentity)
     (selectionSet rest : List Selection) :
     Execution.collectFields schema variableValues parentType source
       (Selection.inlineFragment none [] selectionSet :: rest)
@@ -1050,7 +1052,7 @@ theorem collectFields_inlineFragment_none_directiveFree
 
 theorem collectFields_inlineFragment_some_directiveFree_apply
     (schema : Schema) (variableValues : Execution.VariableValues)
-    (parentType typeCondition : Name) (source : Execution.Value)
+    (parentType typeCondition : Name) (source : Execution.Value ObjectIdentity)
     (selectionSet rest : List Selection) :
     Execution.doesFragmentTypeApplyBool schema parentType source typeCondition = true ->
       Execution.collectFields schema variableValues parentType source
@@ -1065,7 +1067,7 @@ theorem collectFields_inlineFragment_some_directiveFree_apply
 
 theorem collectFields_inlineFragment_some_directiveFree_skip
     (schema : Schema) (variableValues : Execution.VariableValues)
-    (parentType typeCondition : Name) (source : Execution.Value)
+    (parentType typeCondition : Name) (source : Execution.Value ObjectIdentity)
     (selectionSet rest : List Selection) :
     Execution.doesFragmentTypeApplyBool schema parentType source typeCondition = false ->
       Execution.collectFields schema variableValues parentType source
@@ -1080,7 +1082,7 @@ theorem collectFields_inlineFragment_some_directiveFree_skip
 mutual
   theorem collectSelection_namesNodup
       (schema : Schema) (variableValues : Execution.VariableValues)
-      (parentType : Name) (source : Execution.Value)
+      (parentType : Name) (source : Execution.Value ObjectIdentity)
       (selection : Selection) :
       executableGroupNamesNodup
         (Execution.collectSelection schema variableValues parentType source
@@ -1152,7 +1154,7 @@ mutual
 
   theorem collectFields_namesNodup
       (schema : Schema) (variableValues : Execution.VariableValues)
-      (parentType : Name) (source : Execution.Value)
+      (parentType : Name) (source : Execution.Value ObjectIdentity)
       (selectionSet : List Selection) :
       executableGroupNamesNodup
         (Execution.collectFields schema variableValues parentType source
@@ -1173,7 +1175,7 @@ end
 mutual
   theorem collectSelection_wellFormed
       (schema : Schema) (variableValues : Execution.VariableValues)
-      (parentType : Name) (source : Execution.Value)
+      (parentType : Name) (source : Execution.Value ObjectIdentity)
       (selection : Selection) :
       executableGroupsWellFormed
         (Execution.collectSelection schema variableValues parentType source
@@ -1254,7 +1256,7 @@ mutual
 
   theorem collectFields_wellFormed
       (schema : Schema) (variableValues : Execution.VariableValues)
-      (parentType : Name) (source : Execution.Value)
+      (parentType : Name) (source : Execution.Value ObjectIdentity)
       (selectionSet : List Selection) :
       executableGroupsWellFormed
         (Execution.collectFields schema variableValues parentType source
@@ -1276,7 +1278,7 @@ end
 
 theorem collectFields_append
     (schema : Schema) (variableValues : Execution.VariableValues)
-    (parentType : Name) (source : Execution.Value)
+    (parentType : Name) (source : Execution.Value ObjectIdentity)
     (left right : List Selection) :
     Execution.collectFields schema variableValues parentType source
       (left ++ right)
@@ -1301,7 +1303,7 @@ theorem collectFields_append
 
 theorem collectFields_inlineFragment_none_directiveFree_flatten
     (schema : Schema) (variableValues : Execution.VariableValues)
-    (parentType : Name) (source : Execution.Value)
+    (parentType : Name) (source : Execution.Value ObjectIdentity)
     (selectionSet rest : List Selection) :
     Execution.collectFields schema variableValues parentType source
       (Selection.inlineFragment none [] selectionSet :: rest)
@@ -1313,7 +1315,7 @@ theorem collectFields_inlineFragment_none_directiveFree_flatten
 
 theorem collectFields_inlineFragment_some_directiveFree_apply_flatten
     (schema : Schema) (variableValues : Execution.VariableValues)
-    (parentType typeCondition : Name) (source : Execution.Value)
+    (parentType typeCondition : Name) (source : Execution.Value ObjectIdentity)
     (selectionSet rest : List Selection) :
     Execution.doesFragmentTypeApplyBool schema parentType source typeCondition =
       true ->
@@ -1329,7 +1331,7 @@ theorem collectFields_inlineFragment_some_directiveFree_apply_flatten
 
 theorem collectFields_responseName_not_mem_of_responseNameFree
     (schema : Schema) (variableValues : Execution.VariableValues)
-    (parentType : Name) (source : Execution.Value)
+    (parentType : Name) (source : Execution.Value ObjectIdentity)
     (responseName : Name) :
     objectTypeNameBool schema parentType = true ->
       (∃ runtimeType identity,
@@ -1482,7 +1484,7 @@ theorem collectFields_responseName_not_mem_of_responseNameFree
 
 theorem collectFields_field_noDirectives_cons_of_responseName_not_mem
     (schema : Schema) (variableValues : Execution.VariableValues)
-    (parentType : Name) (source : Execution.Value)
+    (parentType : Name) (source : Execution.Value ObjectIdentity)
     (responseName fieldName : Name) (arguments : List Argument)
     (selectionSet rest : List Selection) :
     responseName ∉
@@ -1513,7 +1515,7 @@ theorem collectFields_field_noDirectives_cons_of_responseName_not_mem
 
 theorem collectFields_field_head_exists
     (schema : Schema) (variableValues : Execution.VariableValues)
-    (parentType : Name) (source : Execution.Value)
+    (parentType : Name) (source : Execution.Value ObjectIdentity)
     (responseName fieldName : Name) (arguments : List Argument)
     (selectionSet rest : List Selection) :
     ∃ sourceFields sourceRest,
@@ -1547,7 +1549,7 @@ theorem collectFields_field_head_exists
 
 theorem collectFields_withoutFieldsWithResponseName_directiveFree
     (schema : Schema) (variableValues : Execution.VariableValues)
-    (parentType : Name) (source : Execution.Value)
+    (parentType : Name) (source : Execution.Value ObjectIdentity)
     (responseName : Name) :
     objectTypeNameBool schema parentType = true ->
       (∃ runtimeType identity,
@@ -1713,7 +1715,7 @@ theorem collectFields_withoutFieldsWithResponseName_directiveFree
 
 theorem collectFields_withoutFieldsWithResponseName_eq_sourceRest_of_cons
     (schema : Schema) (variableValues : Execution.VariableValues)
-    (parentType : Name) (source : Execution.Value)
+    (parentType : Name) (source : Execution.Value ObjectIdentity)
     (responseName : Name) (fields : List Execution.ExecutableField)
     (sourceRest : List (Name × List Execution.ExecutableField))
     (selectionSet : List Selection) :
@@ -1747,7 +1749,7 @@ theorem collectFields_withoutFieldsWithResponseName_eq_sourceRest_of_cons
 
 theorem collectFields_withoutFieldsWithResponseName_fieldHead_rest_eq_sourceRest
     (schema : Schema) (variableValues : Execution.VariableValues)
-    (parentType : Name) (source : Execution.Value)
+    (parentType : Name) (source : Execution.Value ObjectIdentity)
     (responseName fieldName : Name) (arguments : List Argument)
     (subselections rest : List Selection)
     (sourceFields : List Execution.ExecutableField)
@@ -1807,7 +1809,7 @@ theorem mergeSelectionSets_append
 
 theorem collectFields_validFieldsWithResponseName_responseSelection
     (schema : Schema) (variableValues : Execution.VariableValues)
-    (parentType : Name) (source : Execution.Value)
+    (parentType : Name) (source : Execution.Value ObjectIdentity)
     (responseName : Name) (selectionSet : List Selection) :
     objectTypeNameBool schema parentType = true ->
       (∃ runtimeType identity,
@@ -1954,7 +1956,7 @@ theorem collectFields_validFieldsWithResponseName_responseSelection
 
 theorem mergeExecutableGroups_nil_left_collectFields
     (schema : Schema) (variableValues : Execution.VariableValues)
-    (parentType : Name) (source : Execution.Value)
+    (parentType : Name) (source : Execution.Value ObjectIdentity)
     (selectionSet : List Selection) :
     executableGroupNamesNodup
       (Execution.mergeExecutableGroups []
@@ -1966,7 +1968,7 @@ theorem mergeExecutableGroups_nil_left_collectFields
 
 theorem mergeExecutableGroups_nil_left_collectFields_eq
     (schema : Schema) (variableValues : Execution.VariableValues)
-    (parentType : Name) (source : Execution.Value)
+    (parentType : Name) (source : Execution.Value ObjectIdentity)
     (selectionSet : List Selection) :
     Execution.mergeExecutableGroups []
       (Execution.collectFields schema variableValues parentType source
@@ -1981,7 +1983,7 @@ theorem mergeExecutableGroups_nil_left_collectFields_eq
 
 theorem collectFields_inlineFragment_some_directiveFree_skip_eq
     (schema : Schema) (variableValues : Execution.VariableValues)
-    (parentType typeCondition : Name) (source : Execution.Value)
+    (parentType typeCondition : Name) (source : Execution.Value ObjectIdentity)
     (selectionSet rest : List Selection) :
     Execution.doesFragmentTypeApplyBool schema parentType source typeCondition = false ->
       Execution.collectFields schema variableValues parentType source
