Tests.lean
@@ -1,2 +1,3 @@
 import Tests.NormalForm
-
+import Tests.Execution
+import Tests.DataModel
